extra lemma red_beta

stlc-norm.fst
@@ -230,22 +230,25 @@ let red_exp_closed t e ty_t f =
   let ExIntro e' h = progress ty_t in
   step_preserves_red' e e' h t ty_t (f e' h)
 
-	     
+val red_beta_induction : t1:typ -> t2:typ -> x:var -> e:exp ->
+               typing (extend empty x t1) e t2 ->
+               (e' : exp -> red t1 e' -> Tot (red t2 (subst_beta_gen x e' e))) ->
+	       e':exp -> red t1 e' -> v:exp -> steps e' v ->
+	       Tot (red t2 (EApp (ELam t1 e) e'))
+let rec red_beta_induction t1 t2 x e ty_t2 f e' red_e' v steps_e'v =
+  match steps_e'v with
+  | Multi_step same_e' e'' same_v step_e'e'' mult_e''v -> 
+     red_exp_closed (EApp (ELam t1 e) e') (TyApp (TyLam t1 ty_t2) (red_typable_empty red_e')) (fun e' (step_ee': step e e') -> magic())
+  | Multi_refl same_e' -> magic()
+				  
 
 val red_beta : t1:typ -> t2:typ -> x:var -> e:exp ->
                typing (extend empty x t1) e t2 ->
                (e' : exp -> red t1 e' -> Tot (red t2 (subst_beta_gen x e' e))) ->
                e' : exp -> red t1 e' -> Tot (red t2 (EApp (ELam t1 e) e'))
 let red_beta t1 t2 x e ty_t2 f e' red_e' =
-  let ExIntro v steps_ev = red_halts red_e' in
-  let rec induction (ter: steps e v) =
-    (match ter with
-     | Multi_step same_e' e'' same_v step_e'e'' mult_e''v -> 
-	red_exp_closed (EApp (ELam t1 e) e') (TyApp (TyLam t1 ty_t2) (red_typable_empty red_e')) (fun e' (step_ee': step e e') -> magic())
-     | Multi_refl same_e' -> magic()
-    )
-  in
-  induction steps_ev
+  let ExIntro v steps_e'v = red_halts red_e' 
+  in red_beta_induction t1 t2 x e ty_t2 f e' red_e' v steps_e'v
 
 
 (* | R_arrow : t1:typ -> t2:typ -> #e:exp -> *)
